interop/klr/klir_common.hpp
@@ -1,0 +1,51 @@
+/*
+Copyright (c) 2025 Amazon.com, Inc. or its affiliates. All Rights Reserved.
+Released under Apache 2.0 license as described in the file LICENSE.
+Authors: Paul Govereau, Sean McLaughlin
+*/
+#pragma once
+#include <memory>
+#include <list>
+
+namespace klr {
+
+#define check_size(s, n)                                                       \
+  static_assert(sizeof(s) == n, "sizeof " #s " unexpected")
+
+typedef uint8_t u8;
+typedef uint64_t u64;
+typedef int64_t i64;
+
+typedef bool Bool;
+typedef int32_t Int;
+typedef uint32_t Nat;
+typedef float Float;
+
+check_size(Float, 4);
+
+using String = std::string;
+
+struct Prop {};
+
+template <class T> using Ptr = std::shared_ptr<T>;
+
+template <class T> Ptr<T> ptr() { return std::make_shared<T>(); }
+
+template <class T> using List = std::list<T>;
+
+// template <class T> List<T> list() { return ptr<std::list<T>>(); }
+
+template <class T> using Option = std::optional<T>;
+
+bool deserialize_tag(FILE *in, u8 *type, u8 *constructor, u8 *len);
+bool deserialize_array_start(FILE *in, u64 *size);
+bool deserialize_option(FILE *in, bool *isSome);
+
+Prop Prop_des(FILE *out);
+Bool Bool_des(FILE *out);
+Nat Nat_des(FILE *out);
+Int Int_des(FILE *out);
+Float Float_des(FILE *out);
+String String_des(FILE *out);
+
+} // namespace klr
