interop/klr/load_test.cpp
@@ -1,0 +1,51 @@
+/*
+A simple example of using the C++ deserialization API.
+This file can be compiled and run with:
+
+# gcc -std=c17 -Wall -c region.c cbor.c
+# g++ --std=c++17 -Wall load_test.cpp klir_serde.cpp klir_common.cpp cbor.o region.o
+# ./a.out test.klr
+*/
+
+#include <iostream>
+#include "klir_ast.hpp"
+#include "klir_serde.hpp"
+
+using namespace std;
+using namespace klr;
+
+int main() {
+  FILE *in = fopen("test.klr", "r");
+  if (!in) {
+    perror("fopen");
+    return 1;
+  }
+
+  Ptr<KLRFile> file = KLRFile_des(in);
+  if (file->major != 0 || file->minor != 0 || file->patch != 12)
+    throw runtime_error("Wrong KLR version");
+
+  cout << "KLR file header, version: " <<
+    file->major << "." <<
+    file->minor << "." <<
+    file->patch << endl;
+
+  Ptr<KLRMetaData> data = KLRMetaData_des(in);
+  cout << "KLR meta data : " <<
+    data->format << endl;
+
+  Ptr<Contents> contents = Contents_des(in);
+  cout << "KLR content type : " <<
+    static_cast<unsigned>(contents->tag) << endl;
+
+  if (contents->tag != Contents::Tag::klir)
+    throw runtime_error("Wrong KLIR content type");
+
+  ContentsKlirWrapper *w = static_cast<ContentsKlirWrapper*>(contents.get());
+  Ptr<Kernel> k = w->kernel;
+  cout << "KLR Kernel : " << k << endl;
+
+  fclose(in);
+
+  return 0;
+}
